tests/lean/run/interactive1.lean
@@ -1,0 +1,32 @@
+def f : nat → nat := λ a, a
+
+@[simp] lemma f_def (a : nat) : f a = a :=
+rfl
+
+def g : nat → nat := λ a, 1 + a
+
+lemma g_def (a : nat) : g a = 1 + a :=
+rfl
+
+example (a b c : nat) : b = 0 → c = 1 → a + b + f c = g (f a) :=
+begin
+  intros h1 h2,
+  simp [h1, h2, g_def, nat.add_comm 1 a]
+end
+
+example (b c : nat) : b = 0 → c = b + 1 → c = 1 :=
+begin
+  intros h1 h2,
+  simp [h1] at h2,
+  assumption
+end
+
+open nat
+
+example (b c : nat) : succ b = succ c → b + 2 = c + 2 :=
+begin
+  intro h,
+  injection h with h', clear h,
+  trace_state,
+  subst h'
+end
